thys/MFOTL_Monitor_Devel/Abstract_Monitor.thy
@@ -13,19 +13,30 @@ text \<open>
   semantics. A first-order specification is described by a finite set of free
   variables and a satisfaction function that defines for every trace the pairs
   of valuations and time-points for which the specification is satisfied.
+  The specification can be restricted to a set of traces to which it applies.
 \<close>
 
 locale fo_spec =
   fixes
     nfv :: nat and fv :: "nat set" and
+    traces :: "'a trace set" and
     sat :: "'a trace \<Rightarrow> 'b list \<Rightarrow> nat \<Rightarrow> bool"
   assumes
     fv_less_nfv: "x \<in> fv \<Longrightarrow> x < nfv" and
-    sat_fv_cong: "(\<And>x. x \<in> fv \<Longrightarrow> v!x = v'!x) \<Longrightarrow> sat \<sigma> v i = sat \<sigma> v' i"
+    sat_fv_cong: "\<sigma> \<in> traces \<Longrightarrow> (\<And>x. x \<in> fv \<Longrightarrow> v!x = v'!x) \<Longrightarrow> sat \<sigma> v i = sat \<sigma> v' i"
 begin
 
 definition verdicts :: "'a trace \<Rightarrow> (nat \<times> 'b tuple) set" where
   "verdicts \<sigma> = {(i, v). wf_tuple nfv fv v \<and> sat \<sigma> (map the v) i}"
+
+definition prefixes :: "'a prefix set" where
+  "prefixes = {\<pi>. \<exists>\<sigma> \<in> traces. prefix_of \<pi> \<sigma>}"
+
+lemma prefix_of_trace[simp, intro]: "\<sigma> \<in> traces \<Longrightarrow> prefix_of \<pi> \<sigma> \<Longrightarrow> \<pi> \<in> prefixes"
+  by (auto simp: prefixes_def)
+
+lemma prefixes_closed[simp, intro]: "\<pi>' \<in> prefixes \<Longrightarrow> \<pi> \<le> \<pi>' \<Longrightarrow> \<pi> \<in> prefixes"
+  using prefix_of_antimono by (auto simp: prefixes_def)
 
 end
 
@@ -38,10 +49,12 @@ text \<open>
 \<close>
 
 locale cosafety_fo_spec = fo_spec +
-  assumes cosafety_lr: "sat \<sigma> v i \<Longrightarrow> \<exists>\<pi>. prefix_of \<pi> \<sigma> \<and> (\<forall>\<sigma>'. prefix_of \<pi> \<sigma>' \<longrightarrow> sat \<sigma>' v i)"
+  assumes cosafety_lr: "\<sigma> \<in> traces \<Longrightarrow> sat \<sigma> v i \<Longrightarrow>
+    \<exists>\<pi>. prefix_of \<pi> \<sigma> \<and> (\<forall>\<sigma>' \<in> traces. prefix_of \<pi> \<sigma>' \<longrightarrow> sat \<sigma>' v i)"
 begin
 
-lemma cosafety: "sat \<sigma> v i \<longleftrightarrow> (\<exists>\<pi>. prefix_of \<pi> \<sigma> \<and> (\<forall>\<sigma>'. prefix_of \<pi> \<sigma>' \<longrightarrow> sat \<sigma>' v i))"
+lemma cosafety: "\<sigma> \<in> traces \<Longrightarrow>
+  sat \<sigma> v i \<longleftrightarrow> (\<exists>\<pi>. prefix_of \<pi> \<sigma> \<and> (\<forall>\<sigma>' \<in> traces. prefix_of \<pi> \<sigma>' \<longrightarrow> sat \<sigma>' v i))"
   using cosafety_lr by blast
 
 end
@@ -57,11 +70,12 @@ text \<open>
 locale monitor = fo_spec +
   fixes M :: "'a prefix \<Rightarrow> (nat \<times> 'b tuple) set"
   assumes
-    mono_monitor: "\<pi> \<le> \<pi>' \<Longrightarrow> M \<pi> \<subseteq> M \<pi>'" and
-    wf_monitor: "(i, v) \<in> M \<pi> \<Longrightarrow> wf_tuple nfv fv v" and
-    sound_monitor: "(i, v) \<in> M \<pi> \<Longrightarrow> prefix_of \<pi> \<sigma> \<Longrightarrow> sat \<sigma> (map the v) i" and
-    complete_monitor: "prefix_of \<pi> \<sigma> \<Longrightarrow> wf_tuple nfv fv v \<Longrightarrow>
-      (\<And>\<sigma>. prefix_of \<pi> \<sigma> \<Longrightarrow> sat \<sigma> (map the v) i) \<Longrightarrow> \<exists>\<pi>'. prefix_of \<pi>' \<sigma> \<and> (i, v) \<in> M \<pi>'"
+    mono_monitor: "\<pi>' \<in> prefixes \<Longrightarrow> \<pi> \<le> \<pi>' \<Longrightarrow> M \<pi> \<subseteq> M \<pi>'" and
+    wf_monitor: "\<pi> \<in> prefixes \<Longrightarrow> (i, v) \<in> M \<pi> \<Longrightarrow> wf_tuple nfv fv v" and
+    sound_monitor: "\<sigma> \<in> traces \<Longrightarrow> (i, v) \<in> M \<pi> \<Longrightarrow> prefix_of \<pi> \<sigma> \<Longrightarrow> sat \<sigma> (map the v) i" and
+    complete_monitor: "\<sigma> \<in> traces \<Longrightarrow> prefix_of \<pi> \<sigma> \<Longrightarrow> wf_tuple nfv fv v \<Longrightarrow>
+      (\<And>\<sigma>'. \<sigma>' \<in> traces \<Longrightarrow> prefix_of \<pi> \<sigma>' \<Longrightarrow> sat \<sigma>' (map the v) i) \<Longrightarrow>
+      \<exists>\<pi>'. prefix_of \<pi>' \<sigma> \<and> (i, v) \<in> M \<pi>'"
 
 text \<open>
   A monitor for a co-safety specification computes precisely the set of all
@@ -73,20 +87,22 @@ abbreviation (in monitor) "M_limit \<sigma> \<equiv> \<Union>{M \<pi> | \<pi>. p
 locale cosafety_monitor = cosafety_fo_spec + monitor
 begin
 
-lemma M_limit_eq: "M_limit \<sigma> = verdicts \<sigma>"
+lemma M_limit_eq:
+  assumes "\<sigma> \<in> traces"
+  shows "M_limit \<sigma> = verdicts \<sigma>"
 proof
   show "\<Union>{M \<pi> | \<pi>. prefix_of \<pi> \<sigma>} \<subseteq> verdicts \<sigma>"
-    by (auto simp: verdicts_def wf_monitor sound_monitor)
+    using assms wf_monitor sound_monitor by (auto simp: verdicts_def)
 next
   show "\<Union>{M \<pi> | \<pi>. prefix_of \<pi> \<sigma>} \<supseteq> verdicts \<sigma>"
     unfolding verdicts_def
   proof safe
     fix i v
     assume "wf_tuple nfv fv v" and "sat \<sigma> (map the v) i"
-    then obtain \<pi> where "prefix_of \<pi> \<sigma> \<and> (\<forall>\<sigma>'. prefix_of \<pi> \<sigma>' \<longrightarrow> sat \<sigma>' (map the v) i)"
-      using cosafety_lr by blast
+    then obtain \<pi> where "prefix_of \<pi> \<sigma> \<and> (\<forall>\<sigma>'\<in>traces. prefix_of \<pi> \<sigma>' \<longrightarrow> sat \<sigma>' (map the v) i)"
+      using assms cosafety_lr by blast
     with \<open>wf_tuple nfv fv v\<close> obtain \<pi>' where "prefix_of \<pi>' \<sigma> \<and> (i, v) \<in> M \<pi>'"
-      using complete_monitor by blast
+      using assms complete_monitor by blast
     then show "(i, v) \<in> \<Union>{M \<pi> | \<pi>. prefix_of \<pi> \<sigma>}"
       by blast
   qed
@@ -102,12 +118,12 @@ text \<open>
   returns for every prefix the time-point up to which all verdicts are computed.
 \<close>
 
-locale progress = fo_spec _ _ sat for sat :: "'a trace \<Rightarrow> 'b list \<Rightarrow> nat \<Rightarrow> bool" +
+locale progress = fo_spec _ _ _ sat for sat :: "'a trace \<Rightarrow> 'b list \<Rightarrow> nat \<Rightarrow> bool" +
   fixes progress :: "'a prefix \<Rightarrow> nat"
   assumes
-    progress_mono: "\<pi> \<le> \<pi>' \<Longrightarrow> progress \<pi> \<le> progress \<pi>'" and
-    ex_progress_ge: "\<exists>\<pi>. prefix_of \<pi> \<sigma> \<and> x \<le> progress \<pi>" and
-    progress_sat_cong: "prefix_of \<pi> \<sigma> \<Longrightarrow> prefix_of \<pi> \<sigma>' \<Longrightarrow> i < progress \<pi> \<Longrightarrow>
+    progress_mono: "\<pi>' \<in> prefixes \<Longrightarrow> \<pi> \<le> \<pi>' \<Longrightarrow> progress \<pi> \<le> progress \<pi>'" and
+    ex_progress_ge: "\<sigma> \<in> traces \<Longrightarrow> \<exists>\<pi>. prefix_of \<pi> \<sigma> \<and> x \<le> progress \<pi>" and
+    progress_sat_cong: "\<sigma> \<in> traces \<Longrightarrow> prefix_of \<pi> \<sigma> \<Longrightarrow> prefix_of \<pi> \<sigma>' \<Longrightarrow> i < progress \<pi> \<Longrightarrow>
       sat \<sigma> v i \<longleftrightarrow> sat \<sigma>' v i"
     \<comment> \<open>The last condition is not necessary to obtain a proper monitor function.
       However, it corresponds to the intuitive understanding of monitor progress,
@@ -117,42 +133,45 @@ begin
 
 definition M :: "'a prefix \<Rightarrow> (nat \<times> 'b tuple) set" where
   "M \<pi> = {(i, v). i < progress \<pi> \<and> wf_tuple nfv fv v \<and>
-    (\<forall>\<sigma>. prefix_of \<pi> \<sigma> \<longrightarrow> sat \<sigma> (map the v) i)}"
+    (\<forall>\<sigma> \<in> traces. prefix_of \<pi> \<sigma> \<longrightarrow> sat \<sigma> (map the v) i)}"
 
-lemma M_alt: "M \<pi> = {(i, v). i < progress \<pi> \<and> wf_tuple nfv fv v \<and>
-    (\<exists>\<sigma>. prefix_of \<pi> \<sigma> \<and> sat \<sigma> (map the v) i)}"
+lemma M_alt: "\<pi> \<in> prefixes \<Longrightarrow> M \<pi> = {(i, v). i < progress \<pi> \<and> wf_tuple nfv fv v \<and>
+    (\<exists>\<sigma> \<in> traces. prefix_of \<pi> \<sigma> \<and> sat \<sigma> (map the v) i)}"
   using ex_prefix_of[of \<pi>]
-  by (auto simp: M_def cong: progress_sat_cong)
+  by (auto simp: prefixes_def M_def cong: progress_sat_cong)
 
 end
 
-sublocale progress \<subseteq> cosafety_monitor _ _ _ M
+sublocale progress \<subseteq> cosafety_monitor _ _ _ _ M
 proof
   fix i v and \<sigma> :: "'a trace"
-  assume "sat \<sigma> v i"
+  assume "\<sigma> \<in> traces" and "sat \<sigma> v i"
   moreover obtain \<pi> where *: "prefix_of \<pi> \<sigma>" "i < progress \<pi>"
-    using ex_progress_ge by (auto simp: less_eq_Suc_le)
+    using \<open>\<sigma> \<in> traces\<close> ex_progress_ge by (auto simp: less_eq_Suc_le)
   ultimately have "sat \<sigma>' v i" if "prefix_of \<pi> \<sigma>'" for \<sigma>'
-    using that by (simp cong: progress_sat_cong)
-  with * show "\<exists>\<pi>. prefix_of \<pi> \<sigma> \<and> (\<forall>\<sigma>'. prefix_of \<pi> \<sigma>' \<longrightarrow> sat \<sigma>' v i)"
+    using \<open>\<sigma> \<in> traces\<close> that progress_sat_cong by blast
+  with * show "\<exists>\<pi>. prefix_of \<pi> \<sigma> \<and> (\<forall>\<sigma>' \<in> traces. prefix_of \<pi> \<sigma>' \<longrightarrow> sat \<sigma>' v i)"
     by blast
 next
   fix \<pi> \<pi>' :: "'a prefix"
-  assume "\<pi> \<le> \<pi>'"
+  assume "\<pi>' \<in> prefixes" and "\<pi> \<le> \<pi>'"
   then show "M \<pi> \<subseteq> M \<pi>'"
     by (auto simp: M_def intro: progress_mono prefix_of_antimono
         elim: order.strict_trans2)
 next
-  fix i v \<pi> and \<sigma> :: "'a trace"
-  assume *: "(i, v) \<in> M \<pi>"
+  fix i v \<pi>
+  assume "\<pi> \<in> prefixes" and "(i, v) \<in> M \<pi>"
   then show "wf_tuple nfv fv v"
-    by (simp add: M_def)
-  assume "prefix_of \<pi> \<sigma>"
-  with * show "sat \<sigma> (map the v) i"
     by (simp add: M_def)
 next
   fix i v \<pi> and \<sigma> :: "'a trace"
-  assume *: "prefix_of \<pi> \<sigma>" "wf_tuple nfv fv v" "\<And>\<sigma>'. prefix_of \<pi> \<sigma>' \<Longrightarrow> sat \<sigma>' (map the v) i"
+  assume "\<sigma> \<in> traces" and "(i, v) \<in> M \<pi>" and "prefix_of \<pi> \<sigma>"
+  then show "sat \<sigma> (map the v) i"
+    by (simp add: M_def)
+next
+  fix i v \<pi> and \<sigma> :: "'a trace"
+  assume *: "\<sigma> \<in> traces" "prefix_of \<pi> \<sigma>" "wf_tuple nfv fv v"
+    "\<And>\<sigma>'. \<sigma>' \<in> traces \<Longrightarrow> prefix_of \<pi> \<sigma>' \<Longrightarrow> sat \<sigma>' (map the v) i"
   show "\<exists>\<pi>'. prefix_of \<pi>' \<sigma> \<and> (i, v) \<in> M \<pi>'"
   proof (cases "i < progress \<pi>")
     case True
@@ -160,9 +179,9 @@ next
   next
     case False
     obtain \<pi>' where **: "prefix_of \<pi>' \<sigma> \<and> i < progress \<pi>'"
-      using ex_progress_ge by (auto simp: less_eq_Suc_le)
+      using \<open>\<sigma> \<in> traces\<close> ex_progress_ge by (auto simp: less_eq_Suc_le)
     then have "\<pi> \<le> \<pi>'"
-      using \<open>prefix_of \<pi> \<sigma>\<close> prefix_of_imp_linear False progress_mono
+      using \<open>\<sigma> \<in> traces\<close> \<open>prefix_of \<pi> \<sigma>\<close> prefix_of_imp_linear False progress_mono
       by (blast intro: order.strict_trans2)
     with * ** show ?thesis
       by (auto simp: M_def intro: prefix_of_antimono)
@@ -200,13 +219,19 @@ abbreviation verdict_filter :: "'b list set \<Rightarrow> (nat \<times> 'b tuple
 
 end
 
-locale sliceable_fo_spec = fo_spec _ _ sat + abstract_slicer relevant_events
+locale sliceable_fo_spec = fo_spec _ _ _ sat + abstract_slicer relevant_events
   for relevant_events :: "'b list set \<Rightarrow> 'a set" and sat :: "'a trace \<Rightarrow> 'b list \<Rightarrow> nat \<Rightarrow> bool" +
-  assumes sliceable: "v \<in> S \<Longrightarrow> sat (slice S \<sigma>) v i \<longleftrightarrow> sat \<sigma> v i"
+  assumes
+    slice_closed[simp, intro]: "\<sigma> \<in> traces \<Longrightarrow> slice S \<sigma> \<in> traces" and
+    sliceable: "\<sigma> \<in> traces \<Longrightarrow> v \<in> S \<Longrightarrow> sat (slice S \<sigma>) v i \<longleftrightarrow> sat \<sigma> v i"
 begin
+
+lemma pslice_closed[simp, intro]: "\<pi> \<in> prefixes \<Longrightarrow> pslice S \<pi> \<in> prefixes"
+  using prefix_of_pmap_\<Gamma> by (fastforce simp: prefixes_def)
 
 lemma union_verdicts_slice:
   assumes part: "\<Union>\<S> = UNIV"
+    and trace: "\<sigma> \<in> traces"
   shows "\<Union>((\<lambda>S. verdict_filter S (verdicts (slice S \<sigma>))) ` \<S>) = verdicts \<sigma>"
 proof safe
   fix S i and v :: "'b tuple"
@@ -217,12 +242,12 @@ proof safe
   then obtain v' where "v' \<in> S" and 1: "\<forall>i\<in>fv. v ! i = Some (v' ! i)"
     using tuple by (auto simp: fv_less_nfv elim: mem_restrE)
   then have "sat (slice S \<sigma>) v' i"
-    using \<open>sat (slice S \<sigma>) (map the v) i\<close> tuple
+    using trace \<open>sat (slice S \<sigma>) (map the v) i\<close> tuple
     by (auto simp: wf_tuple_length fv_less_nfv cong: sat_fv_cong)
   then have "sat \<sigma> v' i"
-    using sliceable[OF \<open>v' \<in> S\<close>] by simp
+    using sliceable[OF trace \<open>v' \<in> S\<close>] by simp
   then have "sat \<sigma> (map the v) i"
-    using tuple 1
+    using trace tuple 1
     by (auto simp: wf_tuple_length fv_less_nfv cong: sat_fv_cong)
   then show "(i, v) \<in> verdicts \<sigma>"
     using tuple by (simp add: verdicts_def)
@@ -237,7 +262,7 @@ next
     using mem_restrI[of "map the v" S nfv fv] tuple
     by (auto simp: wf_tuple_def fv_less_nfv)
   moreover have "sat (slice S \<sigma>) (map the v) i"
-    using \<open>sat \<sigma> (map the v) i\<close> sliceable[OF \<open>map the v \<in> S\<close>] by simp
+    using \<open>sat \<sigma> (map the v) i\<close> sliceable[OF trace \<open>map the v \<in> S\<close>] by simp
   then have "(i, v) \<in> verdicts (slice S \<sigma>)"
     using tuple by (simp add: verdicts_def)
   ultimately show "(i, v) \<in> (\<Union>S\<in>\<S>. verdict_filter S (verdicts (slice S \<sigma>)))"
@@ -251,30 +276,31 @@ text \<open>
   the time-point at which verdicts are output must not change.
 \<close>
 
-locale sliceable_monitor = monitor _ _ sat M + abstract_slicer relevant_events
+locale sliceable_monitor = monitor _ _ _ sat M + abstract_slicer relevant_events
   for relevant_events :: "'b list set \<Rightarrow> 'a set" and sat :: "'a trace \<Rightarrow> 'b list \<Rightarrow> nat \<Rightarrow> bool" and M +
-  assumes sliceable_M: "mem_restr S v \<Longrightarrow> (i, v) \<in> M (pslice S \<pi>) \<longleftrightarrow> (i, v) \<in> M \<pi>"
+  assumes sliceable_M: "\<pi> \<in> prefixes \<Longrightarrow> mem_restr S v \<Longrightarrow> (i, v) \<in> M (pslice S \<pi>) \<longleftrightarrow> (i, v) \<in> M \<pi>"
 begin
 
 lemma union_M_pslice:
   assumes part: "\<Union>\<S> = UNIV"
+    and prefix: "\<pi> \<in> prefixes"
   shows "\<Union>((\<lambda>S. verdict_filter S (M (pslice S \<pi>))) ` \<S>) = M \<pi>"
 proof safe
   fix S i and v :: "'b tuple"
   assume "mem_restr S v" and "(i, v) \<in> M (pslice S \<pi>)"
-  then show "(i, v) \<in> M \<pi>" using sliceable_M by blast
+  then show "(i, v) \<in> M \<pi>" using sliceable_M prefix by blast
 next
   fix i and v :: "'b tuple"
   assume "(i, v) \<in> M \<pi>"
   then have tuple: "wf_tuple nfv fv v"
-    by (rule wf_monitor)
+    using prefix wf_monitor by blast
   from part obtain S where "S \<in> \<S>" and "map the v \<in> S"
     by blast
   then have "mem_restr S v"
     using mem_restrI[of "map the v" S nfv fv] tuple
     by (auto simp: wf_tuple_def fv_less_nfv)
   then have "(i, v) \<in> M (pslice S \<pi>)"
-    using \<open>(i, v) \<in> M \<pi>\<close> sliceable_M by blast
+    using \<open>(i, v) \<in> M \<pi>\<close> sliceable_M prefix by blast
   then show "(i, v) \<in> (\<Union>S\<in>\<S>. verdict_filter S (M (pslice S \<pi>)))"
     using \<open>S \<in> \<S>\<close> \<open>mem_restr S v\<close> by blast
 qed
@@ -287,33 +313,34 @@ text \<open>
 \<close>
 
 locale timed_progress = progress +
-  assumes progress_time_conv: "pts \<pi> = pts \<pi>' \<Longrightarrow> progress \<pi> = progress \<pi>'"
+  assumes progress_time_conv: "\<pi> \<in> prefixes \<Longrightarrow> \<pi>' \<in> prefixes \<Longrightarrow>
+    pts \<pi> = pts \<pi>' \<Longrightarrow> progress \<pi> = progress \<pi>'"
 
 locale sliceable_timed_progress = sliceable_fo_spec + timed_progress
 begin
 
-lemma progress_pslice[simp]: "progress (pslice S \<pi>) = progress \<pi>"
+lemma progress_pslice[simp]: "\<pi> \<in> prefixes \<Longrightarrow> progress (pslice S \<pi>) = progress \<pi>"
   by (simp cong: progress_time_conv)
 
 end
 
-sublocale sliceable_timed_progress \<subseteq> sliceable_monitor _ _ _ _ M
+sublocale sliceable_timed_progress \<subseteq> sliceable_monitor _ _ _ _ _ M
 proof
-  fix S :: "'a list set" and v i \<pi>
-  assume *: "mem_restr S v"
+  fix S :: "'b list set" and v i \<pi>
+  assume *: "\<pi> \<in> prefixes" "mem_restr S v"
   show "(i, v) \<in> M (pslice S \<pi>) \<longleftrightarrow> (i, v) \<in> M \<pi>" (is "?L \<longleftrightarrow> ?R")
   proof
     assume ?L
     with * show ?R
       by (auto 0 4 simp: M_def wf_tuple_def elim!: mem_restrE
           box_equals[OF sliceable sat_fv_cong sat_fv_cong, THEN iffD1, rotated -1]
-          intro: prefix_of_psliceI dest: fv_less_nfv spec[of _ "slice S _"])
+          intro: prefix_of_psliceI dest: fv_less_nfv spec[of _ "slice S _"]) (* SLOW *)
   next
     assume ?R
     with * show ?L
       by (auto 0 4 simp: M_alt wf_tuple_def elim!: mem_restrE
         box_equals[OF sliceable sat_fv_cong sat_fv_cong, THEN iffD2, rotated -1]
-        intro: exI[of _ "slice S _"] prefix_of_psliceI dest: fv_less_nfv)
+        intro: exI[of _ "slice S _"] prefix_of_psliceI dest: fv_less_nfv) (* SLOW *)
   qed
 qed
 
